Example: fixed-size array

src/lowparse/LowParseExample.Aux.fst
@@ -1,5 +1,7 @@
 module LowParseExample.Aux
 
+#reset-options "--using_facts_from '* -FStar.Tactics -FStar.Reflection' --z3rlimit 16 --z3cliopt smt.arith.nl=false --max_fuel 2 --max_ifuel 2"
+
 module LP = LowParse.SLow
 module U8 = FStar.UInt8
 module U16 = FStar.UInt16
@@ -51,6 +53,10 @@ let synth_case_A (z: (U8.t * U8.t)) : Tot (LP.sum_cases t_sum Case_A) =
   in
   res
 
+let synth_case_A_inj () : Lemma
+  (LP.synth_injective synth_case_A)
+= ()
+
 inline_for_extraction
 let synth_case_B (z: (U16.t)) : Tot (LP.sum_cases t_sum Case_B) =
   [@inline_let]
@@ -60,14 +66,20 @@ let synth_case_B (z: (U16.t)) : Tot (LP.sum_cases t_sum Case_B) =
     assert_norm (LP.sum_tag_of_data t_sum res == Case_B)
   in
   res
+
+let synth_case_B_inj () : Lemma
+  (LP.synth_injective synth_case_B)
+= ()
   
 let parse_cases
   (x: LP.sum_key t_sum)
 : Tot (LP.parser LP.parse_u16_kind  (LP.sum_cases t_sum x))
 = match x with
   | Case_A ->
+    synth_case_A_inj ();
     LP.parse_synth (LP.parse_u8 `LP.nondep_then` LP.parse_u8) synth_case_A
   | Case_B ->
+    synth_case_B_inj ();
     LP.parse_synth LP.parse_u16 synth_case_B
 
 inline_for_extraction
@@ -76,6 +88,8 @@ let parse32_cases
 : Tot (LP.parser32 (parse_cases x))
 = match x with
   | Case_A ->
+    [@inline_let]
+    let _ = synth_case_A_inj () in
     LP.parse32_synth
       _
       synth_case_A
@@ -83,6 +97,8 @@ let parse32_cases
       (LP.parse32_nondep_then LP.parse32_u8 LP.parse32_u8)
       ()
   | Case_B ->
+    [@inline_let]
+    let _ = synth_case_B_inj () in
     LP.parse32_synth
       _
       synth_case_B
@@ -104,3 +120,76 @@ let parse32_t
       parse_t
       ()
     )
+
+let cases_of_t_A (x: t) : Lemma
+  (cases_of_t x == Case_A <==> A? x)
+= ()
+
+inline_for_extraction
+let synth_case_A_inv (z: LP.sum_cases t_sum Case_A) : Tot (z: (U8.t * U8.t)) =
+  [@inline_let]
+  let z' : t = z in
+  let _ = cases_of_t_A z' in
+  match z' with
+  | A res -> res
+
+let synth_case_A_inv_correct () : Lemma
+  (LP.synth_inverse synth_case_A synth_case_A_inv)
+= ()
+
+let cases_of_t_B (x: t) : Lemma
+  (cases_of_t x == Case_B <==> B? x)
+= ()
+
+inline_for_extraction
+let synth_case_B_inv (z: LP.sum_cases t_sum Case_B) : Tot (z: U16.t) =
+  [@inline_let]
+  let z' : t = z in
+  let _ = cases_of_t_B z' in
+  match z' with
+  | B res -> res
+
+let synth_case_B_inv_correct () : Lemma
+  (LP.synth_inverse synth_case_B synth_case_B_inv)
+= ()
+
+let serialize_cases
+  (x: LP.sum_key t_sum)
+: Tot (LP.serializer (parse_cases x))
+= match x with
+  | Case_A ->
+    synth_case_A_inj ();
+    synth_case_A_inv_correct ();
+    LP.serialize_ext'
+      _
+      (LP.serialize_synth
+        _
+        synth_case_A
+        (LP.serialize_nondep_then _ LP.serialize_u8 () _ LP.serialize_u8)
+        synth_case_A_inv
+        ()
+      )
+      (parse_cases x)
+  | Case_B ->
+    synth_case_B_inj ();
+    synth_case_B_inv_correct ();
+    LP.serialize_ext'
+      _
+      (LP.serialize_synth
+        LP.parse_u16
+        synth_case_B
+        LP.serialize_u16
+        synth_case_B_inv
+        ()
+      )
+      (parse_cases x)
+
+let serialize_t : LP.serializer parse_t =
+  LP.serialize_sum t_sum LP.serialize_u8 serialize_cases
+
+let parse_t_array : LP.parser _ (LP.array t 18) =
+  LP.parse_array serialize_t 54 18
+
+inline_for_extraction
+let parse32_t_array : LP.parser32 parse_t_array =
+  LP.parse32_array serialize_t parse32_t 54 54ul 18 ()
