src/lowparse/LowParseExample.fst
@@ -1,4 +1,7 @@
 module LowParseExample
 
-let f (input: FStar.Bytes.bytes) : option (LowParseExample.Aux.t * FStar.UInt32.t) =
+let f (input: FStar.Bytes.bytes) : Tot (option (LowParseExample.Aux.t * FStar.UInt32.t)) =
   LowParseExample.Aux.parse32_t input
+
+let g (input: FStar.Bytes.bytes) : Tot (option (LowParse.SLow.array LowParseExample.Aux.t 18 * FStar.UInt32.t)) =
+  LowParseExample.Aux.parse32_t_array input
